wip: terms

Terms.v
@@ -21,6 +21,8 @@ Inductive theory_equal : th -> th -> Prop :=
 (* Something with Op ? *)
 where "x =t= y" := (theory_equal x y).*)
 
+(*Definition GuardedValues := list (Prop * term)*)               
+
 Inductive term : Type :=
 | Theory : th -> term
 | Location : loc -> term
@@ -28,30 +30,132 @@ Inductive term : Type :=
 
 Reserved Notation "x =s= y" (at level 50).
 
-Inductive semantically_equal : relation term :=
-(*| semeq_th : forall (th1 th2 : th), th1 = th2 -> Theory th1 =s= Theory th2
-| semeq_loc : forall (loc1 loc2 : loc), loc1 = loc2 -> Location loc1 =s= Location loc2*)
-| semeq_eq : forall (t1 t2 : term), t1 = t2 -> t1 =s= t2
-| semeq_symm : forall (t1 t2 : term), t1 =s= t2 -> t2 =s= t1
-| semeq_union_nil : forall (l : list (Prop * term)),
-    ~ (fold_left (fun disj x => match x with (p, _) => disj \/ p end) l False)
-    -> Union l =s= Union []
-| semeq_union : forall (t : term) (l : list (Prop * term)),
-    fold_left (fun disj x => match x with (p, t') => disj \/ (p /\ t =s= t') end) l False
-    -> Union l =s= t
-where "x =s= y" := (semantically_equal x y).
+Fixpoint All {X : Type} (p : X -> Prop) (l : list X) : Prop :=
+  match l with
+  | [] => True
+  | (x :: xs) => p x /\ All p xs
+  end.
 
-Lemma semeq_IsSymm : Symmetric semantically_equal.
-Proof. unfold Symmetric. apply semeq_symm. Qed.
+Fixpoint Any {X : Type} (p : X -> Prop) (l : list X) : Prop :=
+  match l with
+  | [] => False
+  | (x :: xs) => p x \/ Any p xs
+  end.
+
+Fixpoint Union_app (ts : term) (g : Prop) (x : term) : term :=
+  match ts with
+  | Union l => Union ((g, x) :: l)
+  | ts => Union []
+  end.
+
+Inductive sem_empty : term -> Prop :=
+| sem_empty_nil: sem_empty (Union [])
+| sem_empty_cons_empty: forall (t ts : term) (g : Prop),
+    sem_empty t -> sem_empty ts -> sem_empty (Union_app ts g t)
+| sem_empty_cons_false_guard: forall (t ts : term) (g : Prop),
+    ~ g -> sem_empty ts -> sem_empty (Union_app ts g t)
+.
+
+Lemma sem_empty_not_theory : forall (t : th), ~ sem_empty (Theory t).
+Proof. unfold not. intros. inversion H; induction ts; inversion H0. Qed.
+
+Lemma sem_empty_not_location : forall (l : loc), ~ sem_empty (Location l).
+Proof. unfold not. intros. inversion H; induction ts; inversion H0. Qed.
+
+Fixpoint sem_equal (t1 : term) :=
+  fix sem_equal1 (t2 : term) :=
+    sem_empty t1 /\
+    sem_empty t2
+    \/ match t1 with
+       | Union l =>
+         fold_left (fun disj x => match x with (p, t) => disj \/ p /\ (sem_equal t t2) end) l False
+       | _ =>
+         match t2 with
+         | Union l =>
+           Any (fun x => match x with (p, t) => p /\ sem_equal1 t end) l (*
+           fold_right (fun x disj => match x with (p, t) => disj \/ p /\ (sem_equal1 t) end) False l*)
+           (*fold_left (fun disj x => match x with (p, t) => disj \/ p /\ (sem_equal1 t) end) l False *)
+         | _ => t1 = t2
+         end
+       end
+where "x =s= y" := (sem_equal x y).
+
+Lemma union_uncons_l : forall (g : Prop) (t x : term) (l : GuardedValues),
+    g /\ t =s= x \/ Union l =s= x <-> Union ((g, t) :: l) =s= x.
+Proof. admit. Admitted.
+
+Lemma union_uncons_r : forall (g : Prop) (t x : term) (l : GuardedValues),
+    x =s= Union ((g, t) :: l) <-> g /\ t =s= x \/ x =s= Union l.
+Proof. admit. Admitted.
+
+Ltac sem_empty_simpl :=
+  try match goal with
+      | [ H : sem_empty (Theory _) |- _ ] => apply sem_empty_not_theory in H; tauto
+      | [ H : sem_empty (Location _) |- _ ] => apply sem_empty_not_location in H; tauto
+      end.
+
+Ltac semeq_simpl :=
+  try match goal with
+  | [ H : Theory _ =s= Theory _ |- _ ] =>
+    destruct H as [[?A ?B] | ?C]; sem_empty_simpl; inversion_clear C
+  | [ H : Location _ =s= Location _ |- _ ] =>
+    destruct H as [[?A ?B] | ?C]; sem_empty_simpl; inversion_clear C
+  | [ H : Location _ =s= Theory _ |- _ ] =>
+    destruct H as [[?A _] | ?C]; sem_empty_simpl; inversion C
+  | [ H : Theory _ =s= Location _ |- _ ] =>
+    destruct H as [[_ ?A] | ?C]; sem_empty_simpl; inversion C
+  | [ H : Theory _ =s= Union [] |- _ ] =>
+    inversion_clear H as [[?A _] | ?C]; sem_empty_simpl
+  | [ H : Location _ =s= Union [] |- _ ] =>
+    inversion_clear H as [[?A _] | ?C]; sem_empty_simpl
+  | [ H : Union [] =s= Theory _ |- _ ] =>
+    inversion_clear H as [[_ ?A] | ?C]; sem_empty_simpl
+  | [ H : Union [] =s= Location _ |- _ ] =>
+    inversion_clear H as [[_ ?A] | ?C]; sem_empty_simpl
+  end;
+try (simpl; tauto).
+
+Lemma semeq_theories : forall (t1 t2 : th), t1 = t2 <-> Theory t1 =s= Theory t2.
+Proof. intros. split; intros; subst; simpl; auto. semeq_simpl. Qed.
+
+Lemma semeq_locations : forall (l1 l2 : loc), l1 = l2 <-> Location l1 =s= Location l2.
+Proof. intros. split; intros; subst; simpl; auto. semeq_simpl. Qed.
+
+Lemma semeq_IsSymm : Symmetric sem_equal.
+Proof. unfold Symmetric. intros. destruct x, y; semeq_simpl.
+       - induction g. semeq_simpl. destruct a. apply union_uncons_l. apply union_uncons_r in H.
+         destruct H; auto.
+       - induction g. semeq_simpl. destruct a. apply union_uncons_l. apply union_uncons_r in H.
+         destruct H; auto.
+       - induction g. semeq_simpl. destruct a. apply union_uncons_r. apply union_uncons_l in H.
+         destruct H; auto.
+       - induction g. semeq_simpl. destruct a. apply union_uncons_r. apply union_uncons_l in H.
+         destruct H; auto.
+       - induction g0.
+         + simpl. left. split. constructor. inversion H as [[A _] | C]. assumption.
+       - induction g.
+         + simpl in *. destruct H as [[_ B] | C].
+           * left. split. assumption. constructor.
+           * admit.
+         + 
+
+Lemma kek : forall (g : Prop) (t' trm : term) (l : GuardedValues),
+    fold_left (fun disj x => match x with (p, t) => disj \/ p /\ (t =s= t') end) ((g, trm) :: l) False = fold_left (fun disj x => match x with (p, t) => disj \/ p /\ (t =s= t') end) l False \/ g /\ trm =s= t'.
+Proof. intros. simpl. admit. Admitted.
+
+Lemma union_cons_simpl : forall (g : Prop) (t x : term) (gv : GuardedValues),
+    Union ((g, t) :: gv) =s= x -> Union gv =s= x \/ g /\ t =s= x.
+Proof. intros. unfold semantically_equal in H; fold semantically_equal in H. simpl in H.
+       simpl. admit. Admitted.
 
 Lemma semeq_IsRefl : Reflexive semantically_equal.
-Proof. unfold Reflexive. intro x. induction x.
-       - constructor. reflexivity.
-       - constructor. reflexivity.
-       - induction l.
-         + apply semeq_union_nil. auto.
-         + apply semeq_union. simpl.
+Proof. unfold Reflexive. intro x. destruct x. simpl; auto. simpl; auto.
+       induction g. simpl; auto. unfold semantically_equal; fold semantically_equal.
+       replace (a :: g) with ([a] ++ g); auto. rewrite fold_left_app.
+       simpl. destruct a. admit. Admitted.
 
-  
+
+(* ----------------------------------Meaningfull lemmas-------------------------------------- *)
+
 Lemma union_True : forall (t : term), Union [(True, t)] =s= t.
-Proof. 
+Proof. intro t. simpl. right. split; auto. apply semeq_IsRefl. Qed.
